vale/code/arch/x64/interop/GenericInterop2.fsti
@@ -44,23 +44,27 @@ let create_initial_vale_state_core
        (stack:b8{mem_roots_p h0 (stack::acc)})
   : GTot va_state =
   let t_state, mem = create_initial_trusted_state_core acc regs xmms taint h0 stack in
-  { ok = TS.(BS.(t_state.state.ok));
-    regs = X64.Vale.Regs.of_fun TS.(BS.(t_state.state.regs));
-    xmms =  X64.Vale.Xmms.of_fun TS.(BS.(t_state.state.xmms));
-    flags = TS.(BS.(t_state.state.flags));
+  { ok = true;
+    regs = X64.Vale.Regs.of_fun (regs_with_stack regs stack);
+    xmms = X64.Vale.Xmms.of_fun xmms;
+    flags = 0; // REVIEW
     mem = to_mem mem;
     memTaint = to_memtaint TS.(t_state.memTaint) }
 
-val core_create_lemma
-       (acc:list b8)
-       (regs:registers)
-       (xmms:xmms_t)
-       (taint:taint_map)
-       (h0:HS.mem)
-       (stack:b8{mem_roots_p h0 (stack::acc)})
+val lemma_create_initial_vale_state_core
+    (acc:list b8)
+    (regs:registers)
+    (xmms:xmms_t)
+    (taint:taint_map)
+    (h0:HS.mem)
+    (stack:b8{mem_roots_p h0 (stack::acc)})
   : Lemma
-      (ensures (fst (create_initial_trusted_state_core acc regs xmms taint h0 stack) ==
-                state_to_S (create_initial_vale_state_core acc regs xmms taint h0 stack)))
+      (requires True)
+      (ensures (
+        let s = create_initial_vale_state_core acc regs xmms taint h0 stack in
+        get_hs s.mem == h0
+      ))
+      [SMTPat (create_initial_vale_state_core acc regs xmms taint h0 stack)]
 
 [@reduce]
 let create_vale_initial_state_t (dom:list vale_type)
